@prefix dct: <http://purl.org/dc/terms/> .
@prefix owl: <http://www.w3.org/2002/07/owl#> .
@prefix rdf: <http://www.w3.org/1999/02/22-rdf-syntax-ns#> .
@prefix xml: <http://www.w3.org/XML/1998/namespace> .
@prefix xsd: <http://www.w3.org/2001/XMLSchema#> .
@prefix foaf: <http://xmlns.com/foaf/0.1/> .
@prefix rdfs: <http://www.w3.org/2000/01/rdf-schema#> .
@prefix voaf: <http://purl.org/vocommons/voaf#> .
@prefix vann: <http://purl.org/vocab/vann/> .
@prefix vs: <http://www.w3.org/2003/06/sw-vocab-status/ns#> .
@prefix cc: <http://creativecommons.org/ns#> .
@prefix fno: <https://w3id.org/function/ontology#> .

@base <https://w3id.org/function/vocabulary/mapping#> .
@prefix : <https://w3id.org/function/vocabulary/mapping#> .

<https://w3id.org/function/vocabulary/mapping#>  rdf:type owl:Ontology ;

                                      rdf:type voaf:Vocabulary;

                                      vann:preferredNamespacePrefix "fnom";

                                      vann:preferredNamespaceUri "https://w3id.org/function/vocabulary/mapping#";

                                      rdfs:label "The Function Ontology - Implementation Mapping vocabulary"@en ;

                                      dct:title "The Function Ontology - Implementation Mapping vocabulary"@en ;

                                      dct:description "The Function Ontology Implementation Mapping vocabulary specifies terms relevant to link FnO models to implementations. The specification is online at https://w3id.org/function/spec"@en;

                                      rdfs:comment """-Version 0.2.0: ReturnMapping
-Version 0.1.0: creation."""@en ;

                                      owl:versionIRI <https://w3id.org/function/vocabulary/mapping/0.2.0> ;

                                      owl:versionInfo "0.2.0" ;

                                      owl:priorVersion "https://w3id.org/function/vocabulary/mapping/0.1.0" ;

                                      rdfs:seeAlso <https://w3id.org/function/spec> ;

                                      dct:modified "2019-05-29"^^xsd:date ;

                                      dct:issued "2019-05-21"^^xsd:date ;

                                      dct:rights "Copyright © Ghent University – imec – IDLab"@en ;

                                      cc:license <http://creativecommons.org/license/by/3.0/> ;

                                      foaf:primaryTopic <https://w3id.org/function/ontology> ;

                                      dct:creator <https://ben.de-meester.org/#me> ;

                                      dct:publisher <https://ben.de-meester.org/#me> .

<https://ben.de-meester.org/#me>  rdf:type foaf:Person ;

                                  foaf:mbox "mailto:Ben.DeMeester@UGent.be";

                                  foaf:name "Ben De Meester"@en ;

                                  rdfs:label "Ben De Meester"@en .

#################################################################
#
#    Object Properties
#
#################################################################

###  https://w3id.org/function/vocabulary/mapping#method-name

:method-name rdf:type rdf:Property ;

        rdfs:label "method name"@en ;

        rdfs:comment "Connects a method name to a method mapping."@en ;

        rdfs:isDefinedBy <https://w3id.org/vocabulary/mapping#> ;

        vs:term_status "testing" ;

        rdfs:domain :StringMethodMapping ;

        rdfs:range xsd:string .

###  https://w3id.org/function/vocabulary/mapping#functionParameter

:functionParameter rdf:type owl:ObjectProperty ;

        rdfs:label "function parameter"@en ;

        rdfs:comment "Connects a function parameter to a parameter mapping."@en ;

        rdfs:isDefinedBy <https://w3id.org/vocabulary/mapping#> ;

        vs:term_status "testing" ;

        rdfs:domain :PositionParameterMapping ;

        rdfs:range fno:Parameter .

###  https://w3id.org/function/vocabulary/mapping#implementationParameterPosition

:implementationParameterPosition rdf:type rdf:Property ;

        rdfs:label "implementation parameter position"@en ;

        rdfs:comment "Connects an implementation parameter position to a parameter mapping."@en ;

        rdfs:isDefinedBy <https://w3id.org/vocabulary/mapping#> ;

        vs:term_status "testing" ;

        rdfs:domain :ParameterMapping ;

        rdfs:range xsd:int .

###  https://w3id.org/function/vocabulary/mapping#implementationProperty

:implementationProperty rdf:type rdf:Property ;

        rdfs:label "implementation property"@en ;

        rdfs:comment "Connects an implementation parameter label to a parameter mapping."@en ;

        rdfs:isDefinedBy <https://w3id.org/vocabulary/mapping#> ;

        vs:term_status "testing" ;

        rdfs:domain :ParameterMapping ;

        rdfs:range xsd:string .

###  https://w3id.org/function/vocabulary/mapping#implementationProperty

:functionOutput rdf:type rdf:Property ;

        rdfs:label "function output"@en ;

        rdfs:comment "Connects a function output to a return mapping."@en ;

        rdfs:isDefinedBy <https://w3id.org/vocabulary/mapping#> ;

        vs:term_status "testing" ;

        rdfs:domain :ReturnMapping ;

        rdfs:range fno:Output .

#################################################################
#
#    Classes
#
#################################################################

###  https://w3id.org/function/vocabulary/mapping#StringMethodMapping

:StringMethodMapping rdf:type owl:Class ;

          rdfs:label "String Method Mapping"@en ;

          rdfs:comment "A string method mapping uses a string to map a method of an fno:Implementation to an fno:Function"@en ;

          vs:term_status "testing" ;

          rdfs:isDefinedBy <https://w3id.org/function/vocabulary/mapping#> ;

          rdfs:subClassOf fno:MethodMapping .

###  https://w3id.org/function/vocabulary/mapping#StringMethodMapping

:PositionParameterMapping rdf:type owl:Class ;

         rdfs:label "Position Parameter Mapping"@en ;

         rdfs:comment "A position parameter mapping uses a position to map a parameter of an fno:Implementation to an fno:Parameter"@en ;

         vs:term_status "testing" ;

         rdfs:isDefinedBy <https://w3id.org/function/vocabulary/mapping#> ;

         rdfs:subClassOf fno:ParameterMapping .

:PropertyParameterMapping rdf:type owl:Class ;

         rdfs:label "Property Parameter Mapping"@en ;

         rdfs:comment "A property parameter mapping uses a property string to map a parameter of an fno:Implementation to an fno:Parameter"@en ;

         vs:term_status "testing" ;

         rdfs:isDefinedBy <https://w3id.org/function/vocabulary/mapping#> ;

         rdfs:subClassOf fno:ParameterMapping .

:DefaultReturnMapping rdf:type owl:Class ;

         rdfs:label "Default Return Mapping"@en ;

         rdfs:comment "A default return mapping links the return value of the method to a fno:Output"@en ;

         vs:term_status "testing" ;

         rdfs:isDefinedBy <https://w3id.org/function/vocabulary/mapping#> ;

         rdfs:subClassOf fno:ReturnMapping .

:ExceptionReturnMapping rdf:type owl:Class ;

         rdfs:label "Exception Return Mapping"@en ;

         rdfs:comment "An exception return mapping links the thrown exception of the method to a fno:Output"@en ;

         vs:term_status "testing" ;

         rdfs:isDefinedBy <https://w3id.org/function/vocabulary/mapping#> ;

         rdfs:subClassOf fno:ReturnMapping .
